<?xml version="1.0"?>
<rdf:RDF xmlns:rdf="http://www.w3.org/1999/02/22-rdf-syntax-ns#"
         xmlns:xsd="http://www.w3.org/2001/XMLSchema#"
         xmlns:rdfs="http://www.w3.org/2000/01/rdf-schema#"
         xmlns:owl="http://www.w3.org/2002/07/owl#"
         xml:base="http://www.semanticweb.org/khunters/ontologies/2016/10/DSMVAutism"
         xmlns="http://www.semanticweb.org/khunters/ontologies/2016/10/DSMVAutism#">

<owl:Ontology rdf:about="http://www.semanticweb.org/khunters/ontologies/2016/10/DSMVAutism">
  <rdfs:comment xml:lang="en">This ontology represents the definition of autism present in DSM-V</rdfs:comment>
  <owl:versionInfo rdf:datatype="http://www.w3.org/2001/XMLSchema#decimal">1.0</owl:versionInfo>
</owl:Ontology>

<owl:ObjectProperty rdf:about="#has_DSMV_Characteristic">
  <rdf:type rdf:resource="http://www.w3.org/2002/07/owl#AsymmetricProperty"/>
  <rdf:type rdf:resource="http://www.w3.org/2002/07/owl#IrreflexiveProperty"/>
  <rdfs:domain rdf:resource="#DSMV_Autistic"/>
  <rdfs:range rdf:resource="#DSMV_Autism_Definition"/>
  <owl:inverseOf rdf:resource="#is_DSMV_Characteristic_Of"/>
</owl:ObjectProperty>

<owl:ObjectProperty rdf:about="#is_DSMV_Characteristic_Of">
  <rdf:type rdf:resource="http://www.w3.org/2002/07/owl#AsymmetricProperty"/>
  <rdf:type rdf:resource="http://www.w3.org/2002/07/owl#IrreflexiveProperty"/>
  <rdfs:domain rdf:resource="#DSMV_Autism_Definition"/>
  <rdfs:range rdf:resource="#DSMV_Autistic"/>
</owl:ObjectProperty>

<owl:ObjectProperty rdf:about="#has_DSMV_Characteristic_A">
  <rdfs:domain rdf:resource="#DSMV_Autistic"/>
  <rdfs:range rdf:resource="#DSMV_Autism_Definition_A"/>
  <rdfs:subPropertyOf rdf:resource="#has_DSMV_Characteristic"/>
  <owl:inverseOf rdf:resource="#is_DSMV_Characteristic_A_Of"/>
</owl:ObjectProperty>

<owl:ObjectProperty rdf:about="#is_DSMV_Characteristic_A_Of">
  <rdfs:domain rdf:resource="#DSMV_Autism_Definition_A"/>
  <rdfs:range rdf:resource="#DSMV_Autistic"/>
  <rdfs:subPropertyOf rdf:resource="#is_DSMV_Characteristic_Of"/>
</owl:ObjectProperty>

<owl:ObjectProperty rdf:about="#has_DSMV_Characteristic_B">
  <rdfs:domain rdf:resource="#DSMV_Autistic"/>
  <rdfs:range rdf:resource="#DSMV_Autism_Definition_B"/>
  <rdfs:subPropertyOf rdf:resource="#has_DSMV_Characteristic"/>
  <owl:inverseOf rdf:resource="#is_DSMV_Characteristic_B_Of"/>
</owl:ObjectProperty>

<owl:ObjectProperty rdf:about="#is_DSMV_Characteristic_B_Of">
  <rdfs:domain rdf:resource="#DSMV_Autism_Definition_B"/>
  <rdfs:range rdf:resource="#DSMV_Autistic"/>
  <rdfs:subPropertyOf rdf:resource="#is_DSMV_Characteristic_Of"/>
</owl:ObjectProperty>

<owl:ObjectProperty rdf:about="#has_DSMV_Characteristic_C">
  <rdf:type rdf:resource="http://www.w3.org/2002/07/owl#FunctionalProperty"/>
  <rdfs:domain rdf:resource="#DSMV_Autistic"/>
  <rdfs:range rdf:resource="#DSMV_Autism_Definition_C"/>
  <rdfs:subPropertyOf rdf:resource="#has_DSMV_Characteristic"/>
  <owl:inverseOf rdf:resource="#is_DSMV_Characteristic_C_Of"/>
</owl:ObjectProperty>

<owl:ObjectProperty rdf:about="#is_DSMV_Characteristic_C_Of">
  <rdfs:domain rdf:resource="#DSMV_Autism_Definition_C"/>
  <rdfs:range rdf:resource="#DSMV_Autistic"/>
  <rdfs:subPropertyOf rdf:resource="#is_DSMV_Characteristic_Of"/>
</owl:ObjectProperty>

<owl:ObjectProperty rdf:about="#has_DSMV_Characteristic_D">
  <rdf:type rdf:resource="http://www.w3.org/2002/07/owl#FunctionalProperty"/>
  <rdfs:domain rdf:resource="#DSMV_Autistic"/>
  <rdfs:range rdf:resource="#DSMV_Autism_Definition_D"/>
  <rdfs:subPropertyOf rdf:resource="#has_DSMV_Characteristic"/>
  <owl:inverseOf rdf:resource="#is_DSMV_Characteristic_D_Of"/>
</owl:ObjectProperty>

<owl:ObjectProperty rdf:about="#is_DSMV_Characteristic_D_Of">
  <rdfs:domain rdf:resource="#DSMV_Autism_Definition_D"/>
  <rdfs:range rdf:resource="#DSMV_Autistic"/>
  <rdfs:subPropertyOf rdf:resource="#is_DSMV_Characteristic_Of"/>
</owl:ObjectProperty>

<owl:ObjectProperty rdf:about="#has_DSMV_Characteristic_E">
  <rdf:type rdf:resource="http://www.w3.org/2002/07/owl#FunctionalProperty"/>
  <rdfs:domain rdf:resource="#DSMV_Autistic"/>
  <rdfs:range rdf:resource="#DSMV_Autism_Definition_E"/>
  <rdfs:subPropertyOf rdf:resource="#has_DSMV_Characteristic"/>
  <owl:inverseOf rdf:resource="#is_DSMV_Characteristic_E_Of"/>
</owl:ObjectProperty>

<owl:ObjectProperty rdf:about="#is_DSMV_Characteristic_E_Of">
  <rdfs:domain rdf:resource="#DSMV_Autism_Definition_E"/>
  <rdfs:range rdf:resource="#DSMV_Autistic"/>
  <rdfs:subPropertyOf rdf:resource="#is_DSMV_Characteristic_Of"/>
</owl:ObjectProperty>

<owl:ObjectProperty rdf:about="#has_Intensity_Level">
  <rdf:type rdf:resource="http://www.w3.org/2002/07/owl#AsymmetricProperty"/>
  <rdf:type rdf:resource="http://www.w3.org/2002/07/owl#IrreflexiveProperty"/>
  <rdfs:domain>
    <owl:Class>
      <owl:unionOf rdf:parseType="Collection">
        <rdf:Description rdf:about="#DSMV_Autism_Definition_A"/>
        <rdf:Description rdf:about="#DSMV_Autism_Definition_B"/>
      </owl:unionOf>
    </owl:Class>
  </rdfs:domain>
  <rdfs:range rdf:resource="#DSMV_Intensity_ValuePartition"/>
</owl:ObjectProperty>

<owl:DatatypeProperty rdf:about="#hasAge">
  <rdf:type rdf:resource="http://www.w3.org/2002/07/owl#FunctionalProperty"/>
  <rdfs:domain rdf:resource="#DSMV_Autistic"/>
  <rdfs:range rdf:resource="http://www.w3.org/2001/XMLSchema#integer"/>
  <rdfs:comment>Age of the Person</rdfs:comment>
</owl:DatatypeProperty>

<owl:DatatypeProperty rdf:about="#hasGender">
  <rdf:type rdf:resource="http://www.w3.org/2002/07/owl#FunctionalProperty"/>
  <rdfs:domain rdf:resource="#DSMV_Autistic"/>
  <rdfs:range rdf:resource="http://www.w3.org/2001/XMLSchema#string"/>
  <rdfs:comment>Gender of the Person</rdfs:comment>
</owl:DatatypeProperty>

<owl:DatatypeProperty rdf:about="#hasIdentificationNumber">
  <rdf:type rdf:resource="http://www.w3.org/2002/07/owl#FunctionalProperty"/>
  <rdfs:domain rdf:resource="#DSMV_Autistic"/>
  <rdfs:range rdf:resource="http://www.w3.org/2001/XMLSchema#integer"/>
  <rdfs:comment>Identification Number of the Person</rdfs:comment>
</owl:DatatypeProperty>

<owl:DatatypeProperty rdf:about="#hasName">
  <rdf:type rdf:resource="http://www.w3.org/2002/07/owl#FunctionalProperty"/>
  <rdfs:domain rdf:resource="#DSMV_Autistic"/>
  <rdfs:range rdf:resource="http://www.w3.org/2001/XMLSchema#string"/>
  <rdfs:comment>Name of the Person</rdfs:comment>
</owl:DatatypeProperty>

<owl:Class rdf:about="#DSMV_Autistic">
  <rdfs:comment xml:lang="en">Person with Severity levels of autism spectrum disorder accordling with DSMV</rdfs:comment>
</owl:Class>

<owl:Class rdf:about="#DSMV_Autism_Definition">
  <rdfs:comment xml:lang="en">Diagnostic and Statistical Manual of Mental Disorders (DSM) is the standard classification of mental disorders used by mental health professionals in the United States and contains a listing of diagnostic criteria for every psychiatric disorder recognized by the U.S. healthcare system.</rdfs:comment>
</owl:Class>

<owl:Class rdf:about="#DSMV_Autism_Definition_A">
  <rdfs:subClassOf rdf:resource="#DSMV_Autism_Definition"/>
  <owl:equivalentClass>
    <owl:Class>
      <owl:unionOf rdf:parseType="Collection">
        <rdf:Description rdf:about="#DSMV_Autism_Definition_A_1"/>
        <rdf:Description rdf:about="#DSMV_Autism_Definition_A_2"/>
        <rdf:Description rdf:about="#DSMV_Autism_Definition_A_3"/>
      </owl:unionOf>
    </owl:Class>
  </owl:equivalentClass>
  <rdfs:comment xml:lang="en">Persistent deficits in social communication and social interaction across multiple contexts, as manifested by the following, currently or by history</rdfs:comment>
</owl:Class>

<owl:Class rdf:about="#DSMV_Autism_Definition_B">
  <rdfs:subClassOf rdf:resource="#DSMV_Autism_Definition"/>
  <owl:equivalentClass>
    <owl:Class>
      <owl:unionOf rdf:parseType="Collection">
        <rdf:Description rdf:about="#DSMV_Autism_Definition_B_1"/>
        <rdf:Description rdf:about="#DSMV_Autism_Definition_B_2"/>
        <rdf:Description rdf:about="#DSMV_Autism_Definition_B_3"/>
        <rdf:Description rdf:about="#DSMV_Autism_Definition_B_4"/>
      </owl:unionOf>
    </owl:Class>
  </owl:equivalentClass>
  <rdfs:comment xml:lang="en">Restricted, repetitive patterns of behavior, interests, or activities, as manifested by at least two of the following, currently or by history</rdfs:comment>
</owl:Class>

<owl:Class rdf:about="#DSMV_Autism_Definition_C">
  <rdfs:subClassOf rdf:resource="#DSMV_Autism_Definition"/>
  <rdfs:comment xml:lang="en">Symptoms must be present in the early developmental period (but may not become fully manifest until social demands exceed limited capacities, or may be masked by learned strategies in later life)</rdfs:comment>
</owl:Class>

<owl:Class rdf:about="#DSMV_Autism_Definition_D">
  <rdfs:subClassOf rdf:resource="#DSMV_Autism_Definition"/>
  <rdfs:comment xml:lang="en">Symptoms cause clinically significant impairment in social, occupational, or other important areas of current functioning</rdfs:comment>
</owl:Class>

<owl:Class rdf:about="#DSMV_Autism_Definition_E">
  <rdfs:subClassOf rdf:resource="#DSMV_Autism_Definition"/>
  <rdfs:comment xml:lang="en">These disturbances are not better explained by intellectual disability (intellectual developmental disorder) or global developmental delay. Intellectual disability and autism spectrum disorder frequently co-occur; to make comorbid diagnoses of autism spectrum disorder and intellectual disability, social communication should be below that expected for general developmental level</rdfs:comment>
</owl:Class>

<owl:Class rdf:about="#DSMV_Intensity_ValuePartition">
  <owl:equivalentClass>
    <owl:Class>
      <owl:unionOf rdf:parseType="Collection">
        <rdf:Description rdf:about="#High_Intensity_Level"/>
        <rdf:Description rdf:about="#Low_Intensity_Level"/>
        <rdf:Description rdf:about="#Medium_Intensity_Level"/>
      </owl:unionOf>
    </owl:Class>
  </owl:equivalentClass>
  <rdfs:comment xml:lang="en">Severity level of impairment of the symptoms described in the definitions of autism on the DSMV</rdfs:comment>
</owl:Class>

<owl:Class rdf:about="#DSMV_Autism_Definition_A_1">
  <rdfs:subClassOf rdf:resource="#DSMV_Autism_Definition_A"/>
  <rdfs:comment xml:lang="en">Deficits in social-emotional reciprocity, ranging, for example, from abnormal social approach and failure of normal back-and-forth conversation; to reduced sharing of interests, emotions, or affect; to failure to initiate or respond to social interactions.</rdfs:comment>
</owl:Class>

<owl:Class rdf:about="#DSMV_Autism_Definition_A_2">
  <rdfs:subClassOf rdf:resource="#DSMV_Autism_Definition_A"/>
  <rdfs:comment xml:lang="en">Deficits in nonverbal communicative behaviors used for social interaction, ranging, for example, from poorly integrated verbal and nonverbal communication; to abnormalities in eye contact and body language or deficits in understanding and use of gestures; to a total lack of facial expressions and nonverbal communication.</rdfs:comment>
</owl:Class>

<owl:Class rdf:about="#DSMV_Autism_Definition_A_3">
  <rdfs:subClassOf rdf:resource="#DSMV_Autism_Definition_A"/>
  <rdfs:comment xml:lang="en">Deficits in developing, maintaining, and understanding relationships, ranging, for example, from difficulties adjusting behavior to suit various social contexts; to difficulties in sharing imaginative play or in making friends; to absence of interest in peers.</rdfs:comment>
</owl:Class>

<owl:Class rdf:about="#DSMV_Autism_Definition_B_1">
  <rdfs:subClassOf rdf:resource="#DSMV_Autism_Definition_B"/>
  <rdfs:comment xml:lang="en">Stereotyped or repetitive motor movements, use of objects, or speech (e.g., simple motor stereotypies, lining up toys or flipping objects, echolalia, idiosyncratic phrases).</rdfs:comment>
</owl:Class>

<owl:Class rdf:about="#DSMV_Autism_Definition_B_2">
  <rdfs:subClassOf rdf:resource="#DSMV_Autism_Definition_B"/>
  <rdfs:comment xml:lang="en">Insistence on sameness, inflexible adherence to routines, or ritualized patterns or verbal nonverbal behavior (e.g., extreme distress at small changes, difficulties with transitions, rigid thinking patterns, greeting rituals, need to take same route or eat food every day).</rdfs:comment>
</owl:Class>

<owl:Class rdf:about="#DSMV_Autism_Definition_B_3">
  <rdfs:subClassOf rdf:resource="#DSMV_Autism_Definition_B"/>
  <rdfs:comment xml:lang="en">Highly restricted, fixated interests that are abnormal in intensity or focus (e.g, strong attachment to or preoccupation with unusual objects, excessively circumscribed or perseverative interest).</rdfs:comment>
</owl:Class>

<owl:Class rdf:about="#DSMV_Autism_Definition_B_4">
  <rdfs:subClassOf rdf:resource="#DSMV_Autism_Definition_B"/>
  <rdfs:comment xml:lang="en">Hyper- or hyporeactivity to sensory input or unusual interests in sensory aspects of the environment (e.g., apparent indifference to pain/temperature, adverse response to specific sounds or textures, excessive smelling or touching of objects, visual fascination with lights or movement).</rdfs:comment>
</owl:Class>

<owl:Class rdf:about="#High_Intensity_Level">
  <rdf:type rdf:resource="http://www.w3.org/2002/07/owl#NamedIndividual"/>
  <rdf:type rdf:resource="#High_Intensity_Level"/>
  <rdfs:subClassOf rdf:resource="#DSMV_Intensity_ValuePartition"/>
  <rdfs:comment xml:lang="en">Defines the High Level of Characteristic</rdfs:comment>
</owl:Class>

<owl:Class rdf:about="#Low_Intensity_Level">
  <rdf:type rdf:resource="http://www.w3.org/2002/07/owl#NamedIndividual"/>
  <rdf:type rdf:resource="#Low_Intensity_Level"/>
  <rdfs:subClassOf rdf:resource="#DSMV_Intensity_ValuePartition"/>
  <rdfs:comment xml:lang="en">Defines the Low Level of Characteristic</rdfs:comment>
</owl:Class>

<owl:Class rdf:about="#Medium_Intensity_Level">
  <rdf:type rdf:resource="http://www.w3.org/2002/07/owl#NamedIndividual"/>
  <rdf:type rdf:resource="#Medium_Intensity_Level"/>
  <rdfs:subClassOf rdf:resource="#DSMV_Intensity_ValuePartition"/>
  <rdfs:comment xml:lang="en">Defines the Medium Level of Characteristic</rdfs:comment>
</owl:Class>

<owl:Class rdf:about="#DSMV_Autistic_Level_1">
  <owl:equivalentClass>
    <owl:Class>
      <owl:intersectionOf rdf:parseType="Collection">
        <rdf:Description rdf:about="#DSMV_Autistic"/>
        <owl:Class>
          <owl:intersectionOf rdf:parseType="Collection">
            <owl:Class>
              <owl:unionOf rdf:parseType="Collection">
                <owl:Restriction>
                  <owl:onProperty rdf:resource="#has_DSMV_Characteristic_A"/>
                  <owl:someValuesFrom>
                    <owl:Class>
                      <owl:intersectionOf rdf:parseType="Collection">
                        <rdf:Description rdf:about="#DSMV_Autism_Definition_A_1"/>
                        <owl:Restriction>
                          <owl:onProperty rdf:resource="#has_Intensity_Level"/>
                          <owl:someValuesFrom rdf:resource="#Low_Intensity_Level"/>
                        </owl:Restriction>
                      </owl:intersectionOf>
                    </owl:Class>
                  </owl:someValuesFrom>
                </owl:Restriction>
                <owl:Restriction>
                  <owl:onProperty rdf:resource="#has_DSMV_Characteristic_A"/>
                  <owl:someValuesFrom>
                    <owl:Class>
                      <owl:intersectionOf rdf:parseType="Collection">
                        <rdf:Description rdf:about="#DSMV_Autism_Definition_A_2"/>
                        <owl:Restriction>
                          <owl:onProperty rdf:resource="#has_Intensity_Level"/>
                          <owl:someValuesFrom rdf:resource="#Low_Intensity_Level"/>
                        </owl:Restriction>
                      </owl:intersectionOf>
                    </owl:Class>
                  </owl:someValuesFrom>
                </owl:Restriction>
                <owl:Restriction>
                  <owl:onProperty rdf:resource="#has_DSMV_Characteristic_A"/>
                  <owl:someValuesFrom>
                    <owl:Class>
                      <owl:intersectionOf rdf:parseType="Collection">
                        <rdf:Description rdf:about="#DSMV_Autism_Definition_A_3"/>
                        <owl:Restriction>
                          <owl:onProperty rdf:resource="#has_Intensity_Level"/>
                          <owl:someValuesFrom rdf:resource="#Low_Intensity_Level"/>
                        </owl:Restriction>
                      </owl:intersectionOf>
                    </owl:Class>
                  </owl:someValuesFrom>
                </owl:Restriction>
              </owl:unionOf>
            </owl:Class>
            <owl:Class>
              <owl:unionOf rdf:parseType="Collection">
                <owl:Restriction>
                  <owl:onProperty rdf:resource="#has_DSMV_Characteristic_B"/>
                  <owl:someValuesFrom>
                    <owl:Class>
                      <owl:intersectionOf rdf:parseType="Collection">
                        <rdf:Description rdf:about="#DSMV_Autism_Definition_B_1"/>
                        <owl:Restriction>
                          <owl:onProperty rdf:resource="#has_Intensity_Level"/>
                          <owl:someValuesFrom rdf:resource="#Low_Intensity_Level"/>
                        </owl:Restriction>
                      </owl:intersectionOf>
                    </owl:Class>
                  </owl:someValuesFrom>
                </owl:Restriction>
                <owl:Restriction>
                  <owl:onProperty rdf:resource="#has_DSMV_Characteristic_B"/>
                  <owl:someValuesFrom>
                    <owl:Class>
                      <owl:intersectionOf rdf:parseType="Collection">
                        <rdf:Description rdf:about="#DSMV_Autism_Definition_B_2"/>
                        <owl:Restriction>
                          <owl:onProperty rdf:resource="#has_Intensity_Level"/>
                          <owl:someValuesFrom rdf:resource="#Low_Intensity_Level"/>
                        </owl:Restriction>
                      </owl:intersectionOf>
                    </owl:Class>
                  </owl:someValuesFrom>
                </owl:Restriction>
                <owl:Restriction>
                  <owl:onProperty rdf:resource="#has_DSMV_Characteristic_B"/>
                  <owl:someValuesFrom>
                    <owl:Class>
                      <owl:intersectionOf rdf:parseType="Collection">
                        <rdf:Description rdf:about="#DSMV_Autism_Definition_B_3"/>
                        <owl:Restriction>
                          <owl:onProperty rdf:resource="#has_Intensity_Level"/>
                          <owl:someValuesFrom rdf:resource="#Low_Intensity_Level"/>
                        </owl:Restriction>
                      </owl:intersectionOf>
                    </owl:Class>
                  </owl:someValuesFrom>
                </owl:Restriction>
              </owl:unionOf>
            </owl:Class>
          </owl:intersectionOf>
        </owl:Class>
      </owl:intersectionOf>
    </owl:Class>
  </owl:equivalentClass>
  <rdfs:comment xml:lang="en">Person that Requiring support</rdfs:comment>
</owl:Class>

<owl:Class rdf:about="#DSMV_Autistic_Level_2">
  <owl:equivalentClass>
    <owl:Class>
      <owl:intersectionOf rdf:parseType="Collection">
        <rdf:Description rdf:about="#DSMV_Autistic"/>
        <owl:Class>
          <owl:intersectionOf rdf:parseType="Collection">
            <owl:Class>
              <owl:unionOf rdf:parseType="Collection">
                <owl:Restriction>
                  <owl:onProperty rdf:resource="#has_DSMV_Characteristic_A"/>
                  <owl:someValuesFrom>
                    <owl:Class>
                      <owl:intersectionOf rdf:parseType="Collection">
                        <rdf:Description rdf:about="#DSMV_Autism_Definition_A_1"/>
                        <owl:Restriction>
                          <owl:onProperty rdf:resource="#has_Intensity_Level"/>
                          <owl:someValuesFrom rdf:resource="#Medium_Intensity_Level"/>
                        </owl:Restriction>
                      </owl:intersectionOf>
                    </owl:Class>
                  </owl:someValuesFrom>
                </owl:Restriction>
                <owl:Restriction>
                  <owl:onProperty rdf:resource="#has_DSMV_Characteristic_A"/>
                  <owl:someValuesFrom>
                    <owl:Class>
                      <owl:intersectionOf rdf:parseType="Collection">
                        <rdf:Description rdf:about="#DSMV_Autism_Definition_A_2"/>
                        <owl:Restriction>
                          <owl:onProperty rdf:resource="#has_Intensity_Level"/>
                          <owl:someValuesFrom rdf:resource="#High_Intensity_Level"/>
                        </owl:Restriction>
                      </owl:intersectionOf>
                    </owl:Class>
                  </owl:someValuesFrom>
                </owl:Restriction>
                <owl:Restriction>
                  <owl:onProperty rdf:resource="#has_DSMV_Characteristic_A"/>
                  <owl:someValuesFrom>
                    <owl:Class>
                      <owl:intersectionOf rdf:parseType="Collection">
                        <rdf:Description rdf:about="#DSMV_Autism_Definition_A_3"/>
                        <owl:Restriction>
                          <owl:onProperty rdf:resource="#has_Intensity_Level"/>
                          <owl:someValuesFrom rdf:resource="#Medium_Intensity_Level"/>
                        </owl:Restriction>
                      </owl:intersectionOf>
                    </owl:Class>
                  </owl:someValuesFrom>
                </owl:Restriction>
              </owl:unionOf>
            </owl:Class>
            <owl:Class>
              <owl:unionOf rdf:parseType="Collection">
                <owl:Restriction>
                  <owl:onProperty rdf:resource="#has_DSMV_Characteristic_B"/>
                  <owl:someValuesFrom>
                    <owl:Class>
                      <owl:intersectionOf rdf:parseType="Collection">
                        <rdf:Description rdf:about="#DSMV_Autism_Definition_B_1"/>
                        <owl:Restriction>
                          <owl:onProperty rdf:resource="#has_Intensity_Level"/>
                          <owl:someValuesFrom rdf:resource="#Medium_Intensity_Level"/>
                        </owl:Restriction>
                      </owl:intersectionOf>
                    </owl:Class>
                  </owl:someValuesFrom>
                </owl:Restriction>
                <owl:Restriction>
                  <owl:onProperty rdf:resource="#has_DSMV_Characteristic_B"/>
                  <owl:someValuesFrom>
                    <owl:Class>
                      <owl:intersectionOf rdf:parseType="Collection">
                        <rdf:Description rdf:about="#DSMV_Autism_Definition_B_2"/>
                        <owl:Restriction>
                          <owl:onProperty rdf:resource="#has_Intensity_Level"/>
                          <owl:someValuesFrom rdf:resource="#Medium_Intensity_Level"/>
                        </owl:Restriction>
                      </owl:intersectionOf>
                    </owl:Class>
                  </owl:someValuesFrom>
                </owl:Restriction>
                <owl:Restriction>
                  <owl:onProperty rdf:resource="#has_DSMV_Characteristic_B"/>
                  <owl:someValuesFrom>
                    <owl:Class>
                      <owl:intersectionOf rdf:parseType="Collection">
                        <rdf:Description rdf:about="#DSMV_Autism_Definition_B_3"/>
                        <owl:Restriction>
                          <owl:onProperty rdf:resource="#has_Intensity_Level"/>
                          <owl:someValuesFrom rdf:resource="#Medium_Intensity_Level"/>
                        </owl:Restriction>
                      </owl:intersectionOf>
                    </owl:Class>
                  </owl:someValuesFrom>
                </owl:Restriction>
              </owl:unionOf>
            </owl:Class>
          </owl:intersectionOf>
        </owl:Class>
      </owl:intersectionOf>
    </owl:Class>
  </owl:equivalentClass>
  <rdfs:comment xml:lang="en">Person that Requiring substantial support</rdfs:comment>
</owl:Class>

<owl:Class rdf:about="#DSMV_Autistic_Level_3">
  <owl:equivalentClass>
    <owl:Class>
      <owl:intersectionOf rdf:parseType="Collection">
        <rdf:Description rdf:about="#DSMV_Autistic"/>
        <owl:Class>
          <owl:intersectionOf rdf:parseType="Collection">
            <owl:Class>
              <owl:unionOf rdf:parseType="Collection">
                <owl:Restriction>
                  <owl:onProperty rdf:resource="#has_DSMV_Characteristic_A"/>
                  <owl:someValuesFrom>
                    <owl:Class>
                      <owl:intersectionOf rdf:parseType="Collection">
                        <rdf:Description rdf:about="#DSMV_Autism_Definition_A_1"/>
                        <owl:Restriction>
                          <owl:onProperty rdf:resource="#has_Intensity_Level"/>
                          <owl:someValuesFrom rdf:resource="#High_Intensity_Level"/>
                        </owl:Restriction>
                      </owl:intersectionOf>
                    </owl:Class>
                  </owl:someValuesFrom>
                </owl:Restriction>
                <owl:Restriction>
                  <owl:onProperty rdf:resource="#has_DSMV_Characteristic_A"/>
                  <owl:someValuesFrom>
                    <owl:Class>
                      <owl:intersectionOf rdf:parseType="Collection">
                        <rdf:Description rdf:about="#DSMV_Autism_Definition_A_2"/>
                        <owl:Restriction>
                          <owl:onProperty rdf:resource="#has_Intensity_Level"/>
                          <owl:someValuesFrom rdf:resource="#High_Intensity_Level"/>
                        </owl:Restriction>
                      </owl:intersectionOf>
                    </owl:Class>
                  </owl:someValuesFrom>
                </owl:Restriction>
                <owl:Restriction>
                  <owl:onProperty rdf:resource="#has_DSMV_Characteristic_A"/>
                  <owl:someValuesFrom>
                    <owl:Class>
                      <owl:intersectionOf rdf:parseType="Collection">
                        <rdf:Description rdf:about="#DSMV_Autism_Definition_A_3"/>
                        <owl:Restriction>
                          <owl:onProperty rdf:resource="#has_Intensity_Level"/>
                          <owl:someValuesFrom rdf:resource="#High_Intensity_Level"/>
                        </owl:Restriction>
                      </owl:intersectionOf>
                    </owl:Class>
                  </owl:someValuesFrom>
                </owl:Restriction>
              </owl:unionOf>
            </owl:Class>
            <owl:Class>
              <owl:unionOf rdf:parseType="Collection">
                <owl:Restriction>
                  <owl:onProperty rdf:resource="#has_DSMV_Characteristic_B"/>
                  <owl:someValuesFrom>
                    <owl:Class>
                      <owl:intersectionOf rdf:parseType="Collection">
                        <rdf:Description rdf:about="#DSMV_Autism_Definition_B_1"/>
                        <owl:Restriction>
                          <owl:onProperty rdf:resource="#has_Intensity_Level"/>
                          <owl:someValuesFrom rdf:resource="#High_Intensity_Level"/>
                        </owl:Restriction>
                      </owl:intersectionOf>
                    </owl:Class>
                  </owl:someValuesFrom>
                </owl:Restriction>
                <owl:Restriction>
                  <owl:onProperty rdf:resource="#has_DSMV_Characteristic_B"/>
                  <owl:someValuesFrom>
                    <owl:Class>
                      <owl:intersectionOf rdf:parseType="Collection">
                        <rdf:Description rdf:about="#DSMV_Autism_Definition_B_2"/>
                        <owl:Restriction>
                          <owl:onProperty rdf:resource="#has_Intensity_Level"/>
                          <owl:someValuesFrom rdf:resource="#High_Intensity_Level"/>
                        </owl:Restriction>
                      </owl:intersectionOf>
                    </owl:Class>
                  </owl:someValuesFrom>
                </owl:Restriction>
                <owl:Restriction>
                  <owl:onProperty rdf:resource="#has_DSMV_Characteristic_B"/>
                  <owl:someValuesFrom>
                    <owl:Class>
                      <owl:intersectionOf rdf:parseType="Collection">
                        <rdf:Description rdf:about="#DSMV_Autism_Definition_B_3"/>
                        <owl:Restriction>
                          <owl:onProperty rdf:resource="#has_Intensity_Level"/>
                          <owl:someValuesFrom rdf:resource="#High_Intensity_Level"/>
                        </owl:Restriction>
                      </owl:intersectionOf>
                    </owl:Class>
                  </owl:someValuesFrom>
                </owl:Restriction>
              </owl:unionOf>
            </owl:Class>
          </owl:intersectionOf>
        </owl:Class>
      </owl:intersectionOf>
    </owl:Class>
  </owl:equivalentClass>
  <rdfs:comment xml:lang="en">Person that Requiring very substantial support</rdfs:comment>
</owl:Class>

<DSMV_Autism_Definition_A_1 rdf:about="#Definition_A_1_hig">
  <rdf:type rdf:resource="http://www.w3.org/2002/07/owl#NamedIndividual"/>
  <has_Intensity_Level rdf:resource="#High_Intensity_Level"/>
  <rdfs:comment xml:lang="en">Instance of de Definition A_1 that represents the symptoms at low level of severity</rdfs:comment>
</DSMV_Autism_Definition_A_1>

<DSMV_Autism_Definition_A_1 rdf:about="#Definition_A_1_low">
  <rdf:type rdf:resource="http://www.w3.org/2002/07/owl#NamedIndividual"/>
  <has_Intensity_Level rdf:resource="#Low_Intensity_Level"/>
  <rdfs:comment xml:lang="en">Instance of de Definition A_1 that represents the symptoms at medium level of severity</rdfs:comment>
</DSMV_Autism_Definition_A_1>

<DSMV_Autism_Definition_A_1 rdf:about="#Definition_A_1_med">
  <rdf:type rdf:resource="http://www.w3.org/2002/07/owl#NamedIndividual"/>
  <has_Intensity_Level rdf:resource="#Medium_Intensity_Level"/>
  <rdfs:comment xml:lang="en">Instance of de Definition A_1 that represents the symptoms at high level of severity</rdfs:comment>
</DSMV_Autism_Definition_A_1>

<DSMV_Autism_Definition_A_2 rdf:about="#Definition_A_2_hig">
  <rdf:type rdf:resource="http://www.w3.org/2002/07/owl#NamedIndividual"/>
  <has_Intensity_Level rdf:resource="#High_Intensity_Level"/>
  <rdfs:comment xml:lang="en">Instance of de Definition A_2 that represents the symptoms at high level of severity</rdfs:comment>
</DSMV_Autism_Definition_A_2>

<DSMV_Autism_Definition_A_2 rdf:about="#Definition_A_2_low">
  <rdf:type rdf:resource="http://www.w3.org/2002/07/owl#NamedIndividual"/>
  <has_Intensity_Level rdf:resource="#Low_Intensity_Level"/>
  <rdfs:comment xml:lang="en">Instance of de Definition A_2 that represents the symptoms at low level of severity</rdfs:comment>
</DSMV_Autism_Definition_A_2>

<DSMV_Autism_Definition_A_2 rdf:about="#Definition_A_2_med">
  <rdf:type rdf:resource="http://www.w3.org/2002/07/owl#NamedIndividual"/>
  <has_Intensity_Level rdf:resource="#Medium_Intensity_Level"/>
  <rdfs:comment xml:lang="en">Instance of de Definition A_2 that represents the symptoms at medium level of severity</rdfs:comment>
</DSMV_Autism_Definition_A_2>

<DSMV_Autism_Definition_A_3 rdf:about="#Definition_A_3_hig">
  <rdf:type rdf:resource="http://www.w3.org/2002/07/owl#NamedIndividual"/>
  <has_Intensity_Level rdf:resource="#High_Intensity_Level"/>
  <rdfs:comment xml:lang="en">Instance of de Definition A_3 that represents the symptoms at high level of severity</rdfs:comment>
</DSMV_Autism_Definition_A_3>

<DSMV_Autism_Definition_A_3 rdf:about="#Definition_A_3_low">
  <rdf:type rdf:resource="http://www.w3.org/2002/07/owl#NamedIndividual"/>
  <has_Intensity_Level rdf:resource="#Low_Intensity_Level"/>
  <rdfs:comment xml:lang="en">Instance of de Definition A_3 that represents the symptoms at high low of severity</rdfs:comment>
</DSMV_Autism_Definition_A_3>

<DSMV_Autism_Definition_A_3 rdf:about="#Definition_A_3_med">
  <rdf:type rdf:resource="http://www.w3.org/2002/07/owl#NamedIndividual"/>
  <has_Intensity_Level rdf:resource="#Medium_Intensity_Level"/>
  <rdfs:comment xml:lang="en">Instance of de Definition A_3 that represents the symptoms at medium level of severity</rdfs:comment>
</DSMV_Autism_Definition_A_3>

<DSMV_Autism_Definition_B_1 rdf:about="#Definition_B_1_hig">
  <rdf:type rdf:resource="http://www.w3.org/2002/07/owl#NamedIndividual"/>
  <has_Intensity_Level rdf:resource="#High_Intensity_Level"/>
  <rdfs:comment xml:lang="en">Instance of de Definition B_1 that represents the symptoms at high level of severity</rdfs:comment>
</DSMV_Autism_Definition_B_1>

<DSMV_Autism_Definition_B_1 rdf:about="#Definition_B_1_low">
  <rdf:type rdf:resource="http://www.w3.org/2002/07/owl#NamedIndividual"/>
  <has_Intensity_Level rdf:resource="#Low_Intensity_Level"/>
  <rdfs:comment xml:lang="en">Instance of de Definition B_1 that represents the symptoms at low level of severity</rdfs:comment>
</DSMV_Autism_Definition_B_1>

<DSMV_Autism_Definition_B_1 rdf:about="#Definition_B_1_med">
  <rdf:type rdf:resource="http://www.w3.org/2002/07/owl#NamedIndividual"/>
  <has_Intensity_Level rdf:resource="#Medium_Intensity_Level"/>
  <rdfs:comment xml:lang="en">Instance of de Definition B_1 that represents the symptoms at medium level of severity</rdfs:comment>
</DSMV_Autism_Definition_B_1>

<DSMV_Autism_Definition_B_2 rdf:about="#Definition_B_2_hig">
  <rdf:type rdf:resource="http://www.w3.org/2002/07/owl#NamedIndividual"/>
  <has_Intensity_Level rdf:resource="#High_Intensity_Level"/>
  <rdfs:comment xml:lang="en">Instance of de Definition B_2 that represents the symptoms at high level of severity</rdfs:comment>
</DSMV_Autism_Definition_B_2>

<DSMV_Autism_Definition_B_2 rdf:about="#Definition_B_2_low">
  <rdf:type rdf:resource="http://www.w3.org/2002/07/owl#NamedIndividual"/>
  <has_Intensity_Level rdf:resource="#Low_Intensity_Level"/>
  <rdfs:comment xml:lang="en">Instance of de Definition B_2 that represents the symptoms at low level of severity</rdfs:comment>
</DSMV_Autism_Definition_B_2>

<DSMV_Autism_Definition_B_2 rdf:about="#Definition_B_2_med">
  <rdf:type rdf:resource="http://www.w3.org/2002/07/owl#NamedIndividual"/>
  <has_Intensity_Level rdf:resource="#Medium_Intensity_Level"/>
  <rdfs:comment xml:lang="en">Instance of de Definition B_2 that represents the symptoms at medium level of severity</rdfs:comment>
</DSMV_Autism_Definition_B_2>

<DSMV_Autism_Definition_B_3 rdf:about="#Definition_B_3_hig">
  <rdf:type rdf:resource="http://www.w3.org/2002/07/owl#NamedIndividual"/>
  <has_Intensity_Level rdf:resource="#High_Intensity_Level"/>
  <rdfs:comment xml:lang="en">Instance of de Definition B_3 that represents the symptoms at high level of severity</rdfs:comment>
</DSMV_Autism_Definition_B_3>

<DSMV_Autism_Definition_B_3 rdf:about="#Definition_B_3_low">
  <rdf:type rdf:resource="http://www.w3.org/2002/07/owl#NamedIndividual"/>
  <has_Intensity_Level rdf:resource="#Low_Intensity_Level"/>
  <rdfs:comment xml:lang="en">Instance of de Definition B_3 that represents the symptoms at low level of severity</rdfs:comment>
</DSMV_Autism_Definition_B_3>

<DSMV_Autism_Definition_B_3 rdf:about="#Definition_B_3_med">
  <rdf:type rdf:resource="http://www.w3.org/2002/07/owl#NamedIndividual"/>
  <has_Intensity_Level rdf:resource="#Medium_Intensity_Level"/>
  <rdfs:comment xml:lang="en">Instance of de Definition B_3 that represents the symptoms at medium level of severity</rdfs:comment>
</DSMV_Autism_Definition_B_3>

<DSMV_Autism_Definition_B_4 rdf:about="#Definition_B_4_hig">
  <rdf:type rdf:resource="http://www.w3.org/2002/07/owl#NamedIndividual"/>
  <has_Intensity_Level rdf:resource="#High_Intensity_Level"/>
  <rdfs:comment xml:lang="en">Instance of de Definition B_4 that represents a symptom at high level of severity</rdfs:comment>
</DSMV_Autism_Definition_B_4>

<DSMV_Autism_Definition_B_4 rdf:about="#Definition_B_4_low">
  <rdf:type rdf:resource="http://www.w3.org/2002/07/owl#NamedIndividual"/>
  <has_Intensity_Level rdf:resource="#Low_Intensity_Level"/>
  <rdfs:comment xml:lang="en">Instance of de Definition B_4 that represents a symptom at low level of severity</rdfs:comment>
</DSMV_Autism_Definition_B_4>

<DSMV_Autism_Definition_B_4 rdf:about="#Definition_B_4_med">
  <rdf:type rdf:resource="http://www.w3.org/2002/07/owl#NamedIndividual"/>
  <has_Intensity_Level rdf:resource="#Medium_Intensity_Level"/>
  <rdfs:comment xml:lang="en">Instance of de Definition B_4 that represents a symptom at medium level of severity</rdfs:comment>
</DSMV_Autism_Definition_B_4>

<DSMV_Autism_Definition_C rdf:about="#Definition_C">
  <rdf:type rdf:resource="http://www.w3.org/2002/07/owl#NamedIndividual"/>
  <rdfs:comment xml:lang="en">Instance of de Definition C that represents the symptoms</rdfs:comment>
</DSMV_Autism_Definition_C>

<DSMV_Autism_Definition_D rdf:about="#Definition_D">
  <rdf:type rdf:resource="http://www.w3.org/2002/07/owl#NamedIndividual"/>
  <rdfs:comment xml:lang="en">Instance of de Definition D that represents the symptoms</rdfs:comment>
</DSMV_Autism_Definition_D>

<DSMV_Autism_Definition_E rdf:about="#Definition_E">
  <rdf:type rdf:resource="http://www.w3.org/2002/07/owl#NamedIndividual"/>
  <rdfs:comment xml:lang="en">Instance of de Definition E that represents the symptoms</rdfs:comment>
</DSMV_Autism_Definition_E>

<owl:AllDisjointClasses>
  <owl:members rdf:parseType="Collection">
    <rdf:Description rdf:about="#DSMV_Autism_Definition_A"/>
    <rdf:Description rdf:about="#DSMV_Autism_Definition_B"/>
    <rdf:Description rdf:about="#DSMV_Autism_Definition_C"/>
    <rdf:Description rdf:about="#DSMV_Autism_Definition_D"/>
    <rdf:Description rdf:about="#DSMV_Autism_Definition_E"/>
  </owl:members>
</owl:AllDisjointClasses>

<owl:AllDisjointClasses>
  <owl:members rdf:parseType="Collection">
    <rdf:Description rdf:about="#DSMV_Autism_Definition_A_1"/>
    <rdf:Description rdf:about="#DSMV_Autism_Definition_A_2"/>
    <rdf:Description rdf:about="#DSMV_Autism_Definition_A_3"/>
  </owl:members>
</owl:AllDisjointClasses>

<owl:AllDisjointClasses>
  <owl:members rdf:parseType="Collection">
    <rdf:Description rdf:about="#DSMV_Autism_Definition_B_1"/>
    <rdf:Description rdf:about="#DSMV_Autism_Definition_B_2"/>
    <rdf:Description rdf:about="#DSMV_Autism_Definition_B_3"/>
    <rdf:Description rdf:about="#DSMV_Autism_Definition_B_4"/>
  </owl:members>
</owl:AllDisjointClasses>

<owl:AllDisjointClasses>
  <owl:members rdf:parseType="Collection">
    <rdf:Description rdf:about="#DSMV_Autistic_Level_1"/>
    <rdf:Description rdf:about="#DSMV_Autistic_Level_2"/>
    <rdf:Description rdf:about="#DSMV_Autistic_Level_3"/>
  </owl:members>
</owl:AllDisjointClasses>

<owl:AllDisjointClasses>
  <owl:members rdf:parseType="Collection">
    <rdf:Description rdf:about="#High_Intensity_Level"/>
    <rdf:Description rdf:about="#Low_Intensity_Level"/>
    <rdf:Description rdf:about="#Medium_Intensity_Level"/>
  </owl:members>
</owl:AllDisjointClasses>


</rdf:RDF>
